loc_buffer null == loc_none

ulib/LowStar.Modifies.fst
@@ -34,7 +34,14 @@ let loc_union_loc_none_l = MG.loc_union_loc_none_l
 
 let loc_union_loc_none_r = MG.loc_union_loc_none_r
 
-let loc_buffer #t b = MG.loc_of_aloc #_ #_ #(B.frameOf b) #(B.as_addr b) (B.abuffer_of_buffer b)
+let loc_buffer #t b =
+  if B.g_is_null b
+  then
+    MG.loc_none
+  else
+    MG.loc_of_aloc #_ #_ #(B.frameOf b) #(B.as_addr b) (B.abuffer_of_buffer b)
+
+let loc_buffer_null t = ()
 
 let loc_addresses = MG.loc_addresses
 
@@ -111,7 +118,9 @@ let loc_disjoint_buffer_addresses #t p preserve_liveness r n =
 
 let loc_disjoint_buffer_regions #t p preserve_liveness r =
   MG.loc_disjoint_regions #_ #cls false preserve_liveness (Set.singleton (B.frameOf p)) r;
-  assert (loc_disjoint (loc_regions false (Set.singleton (B.frameOf p))) (loc_regions preserve_liveness r))
+  loc_includes_region_buffer false (Set.singleton (B.frameOf p)) p;
+  loc_includes_refl (loc_regions preserve_liveness r);
+  MG.loc_disjoint_includes (loc_regions false (Set.singleton (B.frameOf p))) (loc_regions preserve_liveness r) (loc_buffer p) (loc_regions preserve_liveness r)
 
 let loc_disjoint_regions = MG.loc_disjoint_regions #_ #cls
 
@@ -122,8 +131,13 @@ let modifies_live_region = MG.modifies_live_region
 let modifies_mreference_elim = MG.modifies_mreference_elim
 
 let modifies_buffer_elim #t1 b p h h' =
+  if B.g_is_null b
+  then
+    assert (B.as_seq h b `Seq.equal` B.as_seq h' b)
+  else begin
     MG.modifies_aloc_elim #_ #cls #(B.frameOf b) #(B.as_addr b) (B.abuffer_of_buffer b) p h h' ;
     B.abuffer_preserved_elim b h h'
+  end
 
 let modifies_refl = MG.modifies_refl
 
@@ -154,16 +168,22 @@ let region_liveness_insensitive_address_liveness_insensitive =
 let modifies_liveness_insensitive_mreference = MG.modifies_preserves_liveness
 
 let modifies_liveness_insensitive_buffer l1 l2 h h' #t x =
-  B.liveness_preservation_intro h h' x (fun t' pre r ->
-    MG.modifies_preserves_liveness_strong l1 l2 h h' r (B.abuffer_of_buffer x)
-  )
+  if B.g_is_null x
+  then ()
+  else
+    B.liveness_preservation_intro h h' x (fun t' pre r ->
+      MG.modifies_preserves_liveness_strong l1 l2 h h' r (B.abuffer_of_buffer x)
+    )
 
 let modifies_liveness_insensitive_region = MG.modifies_preserves_region_liveness
 
 let modifies_liveness_insensitive_region_mreference = MG.modifies_preserves_region_liveness_reference
 
 let modifies_liveness_insensitive_region_buffer l1 l2 h h' #t x =
-  MG.modifies_preserves_region_liveness_aloc l1 l2 h h' #(B.frameOf x) #(B.as_addr x) (B.abuffer_of_buffer x)
+  if B.g_is_null x
+  then ()
+  else
+    MG.modifies_preserves_region_liveness_aloc l1 l2 h h' #(B.frameOf x) #(B.as_addr x) (B.abuffer_of_buffer x)
 
 let modifies_trans = MG.modifies_trans
 
@@ -195,7 +215,12 @@ let modifies_0_modifies h1 h2 =
     (fun t pre b -> B.modifies_0_mreference #t #pre h1 h2 b)
 
 let modifies_1_modifies #t b h1 h2 =
-  MG.modifies_intro (loc_buffer b) h1 h2
+  if B.g_is_null b
+  then begin
+    B.modifies_1_null b h1 h2;
+    modifies_0_modifies h1 h2
+  end else
+   MG.modifies_intro (loc_buffer b) h1 h2
     (fun r -> B.modifies_1_live_region b h1 h2 r)
     (fun t pre p ->
       loc_disjoint_sym (loc_mreference p) (loc_buffer b);
